Pearlite example

examples/pearlite-example/src/pearlite_example.rs
@@ -6,10 +6,8 @@ use hacspec_lib::*;
 #[cfg(not(feature = "hacspec"))]
 use creusot_contracts::{ensures, requires};
 
+#[requires(x == y)]
 #[ensures(result == true)]
-#[cfg(test)]
-#[proof]
-#[quickcheck]
 pub fn ensure_something (x : u8, y : u8) -> bool {
     x == y
 }
