coq/_vc/Pearlite_Example.v
@@ -6,18 +6,14 @@ Import List.ListNotations.
 Open Scope Z_scope.
 Open Scope bool_scope.
 Open Scope hacspec_scope.
-From QuickChick Require Import QuickChick.
-Require Import QuickChickLib.
 Require Import Hacspec_Lib.
 
-Definition ensure_something (x_0 : int8) (y_1 : int8)  : bool :=
+Definition ensure_something (x_0 : int8) (y_1 : int8)  `{x_0 = y_1} : bool :=
   (x_0) =.? (y_1).
 
 Theorem ensures_ensure_something : forall result_2 (x_0 : int8) (y_1 : int8),
- @ensure_something x_0 y_1 = result_2 ->
+ forall {H_0 : x_0 = y_1},
+ @ensure_something x_0 y_1 H_0 = result_2 ->
  result_2 = true.
  Proof. Admitted.
-(*QuickChick (
-  forAll g_int8 (fun x_0 : int8 =>forAll g_int8 (fun y_1 : int8 =>ensure_something x_0 y_1))).*)
-
 
